execution/examples/EIP20Token_Buggy.v
@@ -1,0 +1,99 @@
+(*
+  A buggy version of the EIP20/ERC20 token implementation where transfer_from incorrectly updates balances whenever sender=receiver.
+  This mimics the vulnerability of iToken, as discovered in https://bzx.network/blog/incident
+*)
+
+From Coq Require Import ZArith.
+From Coq Require Import Morphisms.
+Require Import Monads.
+Require Import Extras.
+Require Import Containers.
+Require Import Automation.
+Require Import EIP20Token.
+From RecordUpdate Require Import RecordUpdate.
+From Coq Require Import List.
+Require Import Serializable.
+Require Import Blockchain.
+
+Import ListNotations.
+Import RecordSetNotations.
+
+Section EIP20Token_Buggy.
+  Context {BaseTypes : ChainBase}.
+  Set Primitive Projections.
+  Set Nonrecursive Elimination Schemes.
+
+  Open Scope N_scope.
+  Existing Instance state_settable.
+  Existing Instance setup_settable.
+
+  (* The delegate tries to transfer <amount> tokens from <from> to <to>.
+   Succeeds if <from> has indeed allowed the delegate to spend at least <amount> tokens on its behalf. *)
+  Local Open Scope bool_scope.
+  Definition transfer_from_buggy (delegate : Address)
+       (from : Address)
+       (to : Address)
+       (amount : TokenValue)
+       (state : State) : option State :=
+  do from_allowances_map <- FMap.find from state.(allowances) ;
+  do delegate_allowance <- FMap.find delegate from_allowances_map ;
+  let from_balance := with_default 0 (FMap.find from state.(balances)) in
+  (* Bug starts here! to_balance is calculated too early! *)
+  let to_balance := with_default 0 (FMap.find to state.(balances)) in
+  if ((delegate_allowance <? amount) && negb (from =? to)%address) || (from_balance <? amount)
+  then None
+  else let new_allowances := FMap.add delegate (delegate_allowance - amount) from_allowances_map in
+       let new_balances := FMap.add from (from_balance - amount) state.(balances) in
+       (* Bug here! new balance of 'to' is calculated from to_balance. The commented line below is the correct implementation. *)
+       let new_balances := FMap.add to (to_balance + amount) new_balances in
+       (* let new_balances := FMap.partial_alter (fun balance => Some (with_default 0 balance + amount)) to new_balances in *)
+       Some (state<|balances := new_balances|><|allowances ::= FMap.add from new_allowances|>).
+
+  Definition init_buggy := EIP20Token.init. 
+
+  Open Scope Z_scope.
+  Definition receive_buggy (chain : Chain)
+       (ctx : ContractCallContext)
+       (state : State)
+       (maybe_msg : option Msg)
+    : option (State * list ActionBody) :=
+    let sender := ctx.(ctx_from) in
+    let without_actions := option_map (fun new_state => (new_state, [])) in
+    (* Only allow calls with no money attached *)
+    if ctx.(ctx_amount) >? 0
+    then None
+    else match maybe_msg with
+   | Some (transfer_from from to amount) => without_actions (transfer_from_buggy sender from to amount state)
+   | _ => EIP20Token.receive chain ctx state maybe_msg 
+   end.
+  Close Scope Z_scope.
+
+  Ltac solve_contract_proper :=
+    repeat
+      match goal with
+      | [|- ?x _  = ?x _] => unfold x
+      | [|- ?x _ _ = ?x _ _] => unfold x
+      | [|- ?x _ _ _ = ?x _ _ _] => unfold x
+      | [|- ?x _ _ _ _ = ?x _ _ _ _] => unfold x
+      | [|- ?x _ _ _ _ = ?x _ _ _ _] => unfold x
+      | [|- ?x _ _ _ _ _ = ?x _ _ _ _ _] => unfold x
+      | [|- Some _ = Some _] => f_equal
+      | [|- pair _ _ = pair _ _] => f_equal
+      | [|- (if ?x then _ else _) = (if ?x then _ else _)] => destruct x
+      | [|- match ?x with | _ => _ end = match ?x with | _ => _ end ] => destruct x
+      | [H: ChainEquiv _ _ |- _] => rewrite H in *
+      | _ => subst; auto
+      end.
+
+  Lemma init_buggy_proper :
+    Proper (ChainEquiv ==> eq ==> eq ==> eq) init_buggy.
+  Proof. repeat intro; solve_contract_proper. Qed.
+
+  Lemma receive_buggy_proper :
+    Proper (ChainEquiv ==> eq ==> eq ==> eq ==> eq) receive_buggy.
+  Proof. repeat intro; solve_contract_proper. Qed.
+
+  Definition contract : Contract Setup Msg State :=
+    build_contract init_buggy init_buggy_proper receive_buggy receive_buggy_proper.
+
+End EIP20Token_Buggy.
